%!TEX program = pdflatex
\documentclass[UTF8]{article}

\usepackage[UTF8]{ctex}
\usepackage{amsmath}
\usepackage{enumerate}
\usepackage{amssymb}
\usepackage{graphicx}
\usepackage{booktabs}
 
\title{Homework 11.02}
\author{SA18225036 陈旻}
\date{}
\begin{document}
\maketitle
\section{Question 47}
\paragraph{Question}
Solve the recurrence relation $ h_{n} = 8h_{n - 1} - 16h_{n - 2} $, $ (n \geq 2) $ with initial values $ h_{0} = -1 $ and $ h_{1} = 0 $.
\paragraph{Answer}
    ~\\
    Observe $ x^{2} - 8x + 16 = (x - 4)^{2} $ \\
    Therefore the general solution is
    $$ h_{n} = (a + bn)4^{n} \quad n = 0,1,2,\dots $$
    Using $ h_{0} = -1,h_{1} = 0 $, we obtain $ a = -1 , b = 1 $, Therefore
    $$ h_{n} = (n - 1)4^{n} \quad n = 0,1,2,\dots $$



\section{Question 48}
\paragraph{Question}
Solve the nonhomogeneous recurrence relation
$$ h_{n} = 2h_{n-1} + n , (n \geq 1) , h_{0} = 1.$$
\paragraph{Answer}
~\\
We hunt for solutions of the form
$$ h_{n} = a2^{n} + bn +c \quad n = 0,1,2,\dots $$
Using $ h_{0} = 1, h_{1} = 3, h_{2} = 8 $ \\
We find that $ a = 3, b = -1, c = -2 $ \\
We now verify that
$$ h_{n} = 3 * 2^{n} -n - 2 \quad n = 0,1,2, \dots $$
For $ n \geq 0 $ define $ H_{n} = 3 * 2^{n} - n - 2 $. One checks that $ H_{0} = 1 $ and
$$ H_{n} = 2H_{n - 1} + n \quad n = 1,2,3, \dots $$
Therefore $ h_{n} = H_{n} $ for $ n \geq 0 $
\section{Question 49}
\paragraph{Question}
Solve the following recurrence relations by using the method of generating functions as described in Section 7.5, 
\begin{enumerate}[(a)]
    \item $ h_{n} = 4h_{n - 2} , (n \geq 2); \quad h_{0} = 0, h_{1} = 1 $
    \item $ h_{n} = h_{n - 1} + h_{n - 2}, (n \geq 2); \quad h_{0} = 0, h_{1} = 3 $
    \item $ h_{n} = h_{n - 1} + 9h_{n - 2} - 9h_{n - 3}, (n \geq 3); \quad h_{0} = 0, h_{1} = 1, h_{2} = 2 $
    \item $ h_{n} = 8h_{n - 1} - 16h_{n - 2}, (n \geq 2); \quad h_{0} = -1, h_{1} = 0 $
    \item $ h_{n} = 3h_{n - 2} - 2h_{n - 3}, (n \geq 3); \quad h_{0} = 1, h_{1} = 0, h_{2} = 0 $
    \item $ h_{n} = 5h_{n - 1} - 6h_{n - 2} - 4h_{n - 3} + 8h_{n - 4}, (n \geq 4); \quad h_{0} = 0, h_{1} = 1, h_{2} = 1, h_{3} = 2 $
\end{enumerate}
\paragraph{Answer}
~\\
Define $ g(x) = \sum_{n = 0}^{\infty}h_{n}x^{n} $. Note that $ x^{r}g(x) = \sum_{n = r}^{\infty}h_{n - r}x^{n} $ for $ r \geq 0 $
\begin{enumerate}[(a)]
    \item Using the given information on $ h_{n} $ we find
          $$ g(x)  = x + 4x^{2}g(x) $$
          Therefore
          \begin{equation}
          \begin{aligned}
          g(x) &= \frac{x}{1 - 4x^{2}} \\
          &= \frac{1}{4(1 - 2x)} - \frac{1}{4(1 + 2x)} \\
          &= \sum_{n = 0}^\infty \frac{2^{n} - {(-2)}^{n}}{4} x^{n}
          \nonumber
          \end{aligned}
          \end{equation}
          Therefore
          $$ h_{n} = \frac{2^{n} - {(-2)}^{n}}{4} \quad n=0,1,2, \dots $$
    \item Abbreviate $ r = \frac{1 + \sqrt{5}}{2} $, \quad $ s = \frac{1 - \sqrt{5}}{2} $ \\
          Using the given information on $ h_{n} $ we find
          $$ g(x)(1 - x - x^2)  = 1 + 2x $$
          Therefore
          \begin{equation}
          \begin{aligned}
          g(x) &= \frac{1 + 2x}{1 - x - x^2} \\
          &= \frac{r}{1 - rx} - \frac{s}{1 - sx} \\
          &= \sum_{n = 0}^\infty (r^{n + 1} + s^{n + 1}) x^{n}
          \nonumber
          \end{aligned}
          \end{equation}
          Therefore
          $$ h_{n} = r^{n + 1} + s^{n + 1} \quad n=0,1,2, \dots $$
    \item Using the given information on $ h_{n} $ we find
          $$ g(x)(1 -x - 9x^2 + 9x^3)  = x + x^2 $$
          Consequently
          \begin{equation}
          \begin{aligned}
          g(x) &= \frac{x + x^2}{1 -x - 9x^2 + 9x^3} \\
          &= \frac{1}{3(1 - 3x)} - \frac{1}{12(1 + 3x)} - \frac{1}{4(1 - x)} \\
          &= \sum_{n = 0}^\infty \frac{4*3^{n} - {(-3)}^{n} - 3}{12} x^{n}
          \nonumber
          \end{aligned}
          \end{equation}
          Therefore
          $$ h_{n} = \frac{4*3^{n} - {(-3)}^{n} - 3}{12} x^{n} \quad n=0,1,2, \dots $$
    \item Using the given information on $ h_{n} $ we find
          $$ g(x)(1 - 8x + 16x^2)  = 8x - 1 $$
          Consequently
          \begin{equation}
          \begin{aligned}
          g(x) &= \frac{8x - 1}{1 - 8x + 16x^2} \\
          &= \frac{8x - 1}{(1 - 4x)^2} \\
          &= (8x - 1)\sum_{n = 0}^\infty (n + 1)4^n x^n \\
          &= \sum_{n = 0}^\infty (n - 1)4^n x^n
          \nonumber
          \end{aligned}
          \end{equation}
          Therefore
          $$ h_{n} = (n - 1)4^n \quad n=0,1,2, \dots $$
    \item Therefore
          \begin{equation}
          \begin{aligned}
          g(x) &= \frac{1 - 3x^2}{1 - 3x^2 + 2x^3} \\
          &= \frac{\frac{14}{9}}{1 - x} - \frac{\frac{2}{3}}{(1 - x)^2} + \frac{\frac{1}{9}}{1 + 2x} \\
          &= \sum_{n = 0}^\infty [\frac{14}{9} - \frac{2}{3}(n + 1) + \frac{1}{9}(-2)^n] x^{n}
          \nonumber
          \end{aligned}
          \end{equation}
          Therefore
          $$ h_{n} = \frac{14}{9} - \frac{2}{3}(n + 1) + \frac{1}{9}(-2)^n \quad n=0,1,2, \dots $$
    \item Therefore
          \begin{equation}
          \begin{aligned}
          g(x) &= \frac{x - 4x^2 = 3x^3}{1 - 5x + 6x^2 + 4x^3 - 8x^4} \\
          &= \frac{\frac{17}{4 * 27}}{1 - 2x} - \frac{\frac{2}{9}}{(1 - 2x)^2} -\frac{\frac{1}{12}}{(1 - 2x)^3} - \frac{\frac{8}{27}}{1 + x}\\
          &= \sum_{n = 0}^\infty [\frac{17}{4 * 27} + \frac{2}{9}(n + 1) - \frac{(n + 2)(n + 1)}{24}] 2^n x^{n} - \frac{8}{27} \sum_{n = 0}^\infty (-1)^n x^n
          \nonumber
          \end{aligned}
          \end{equation}
          Therefore
          $$ h_{n} = [\frac{17}{4 * 27} + \frac{2}{9}(n + 1) - \frac{(n + 2)(n + 1)}{24}] x^{n} - \frac{8}{27}  (-1)^n \quad n=0,1,2, \dots $$
\end{enumerate}
\section{Question 50}
\paragraph{Question}
Let $ h_{0}, h_{1}, h_{2}, \cdots ,h_{n}, \cdots $ be the sequence dened by $ h_{n} = \begin{pmatrix} n \\ 2 \end{pmatrix} $, $ (n \geq 0) $. Determine the generating function for the sequence.
\paragraph{Answer}
~\\
We want $ g(x) = \sum_{n = 0}^\infty \begin{pmatrix} n \\ 2 \end{pmatrix} x^n $
The first two terms are zero so we can rewrite the sum as: 
$$ g(x) = \sum_{n = 2}^\infty \begin{pmatrix} n \\ 2 \end{pmatrix} x^n $$
lets add $ 3-1 $: 
$$ \sum_{n = 0}^\infty \begin{pmatrix} n + 3 - 1 \\ 2 \end{pmatrix} x^{n + 2} $$      
factor out $ x^2 $ , $ x^2 \sum_{n = 0}^\infty \begin{pmatrix} n + 3 - 1 \\ 2 \end{pmatrix} x^{n} $
so we have the generating function to be \\
$$ \frac{x^2}{(1 - x)^3} $$
\end{document}